added more about node validity

Systems/Address.v
@@ -2,7 +2,7 @@ From Coq Require Import Lia List ssrbool.
 
 Module Type NetAddr.
 
-(* TODO a better approach is to make Address a finite type; lists are awkward here *)
+(* TODO validity and NoDup checks are everywhere. Consider changing the address type into a finite type eventually *)
 
 (* how about simply letting addr be a number within some range? any other things to notice here? *)
 (* TODO relate this with Byzantine assumption *)
@@ -12,6 +12,8 @@ Parameter Address_eqdec : forall (a1 a2 : Address), {a1 = a2} + {a1 <> a2}.
 
 Parameter is_byz : Address -> bool.
 Parameter valid_nodes : list Address.
+
+Axiom valid_nodes_NoDup : NoDup valid_nodes.
 
 Definition N := length valid_nodes.
 Parameter t0 : nat.
@@ -29,7 +31,10 @@ Qed.
 
 (* TODO if we want properties about quorum, we need to quantify t0 here *)
 
+(* make valid_node explicitly decidable *)
+
 Definition valid_node n := In n valid_nodes.
+Definition is_valid_node n := In_dec Address_eqdec n valid_nodes.
 
 Axiom byz_is_valid : forall n, is_byz n -> valid_node n.
 
